finish computational portions of operations needed for Montgomery, and sketch out some of the proofs as discussed in #157

src/Arithmetic/Saturated.v
@@ -103,6 +103,70 @@ check confirms our result.
 
  ***)
 
+Module Associational.
+  Section Associational.
+    Context {mul_split : Z -> Z -> Z -> Z * Z} (* first argument is where to split output; [mul_split s x y] gives ((x * y) mod s, (x * y) / s) *)
+            {mul_split_mod : forall s x y,
+                fst (mul_split s x y)  = (x * y) mod s}
+            {mul_split_div : forall s x y,
+                snd (mul_split s x y)  = (x * y) / s}
+            .
+
+    Definition multerm_cps s (t t' : B.limb) {T} (f:list B.limb ->T) :=
+      dlet xy := mul_split s (snd t) (snd t') in 
+      f ((fst t * fst t', fst xy) :: (fst t * fst t' * s, snd xy) :: nil).
+
+    Definition multerm s t t' := multerm_cps s t t' id.
+    Lemma multerm_id s t t' T f :
+      @multerm_cps s t t' T f = f (multerm s t t').
+    Proof. reflexivity. Qed.
+    Hint Opaque multerm : uncps.
+    Hint Rewrite multerm_id : uncps.
+
+    Definition mul_cps s (p q : list B.limb) {T} (f : list B.limb -> T) :=
+      flat_map_cps (fun t => @flat_map_cps _ _ (multerm_cps s t) q) p f.
+
+    Definition mul s p q := mul_cps s p q id.
+    Lemma mul_id s p q T f : @mul_cps s p q T f = f (mul s p q).
+    Proof. cbv [mul mul_cps]. autorewrite with uncps. reflexivity. Qed.
+    Hint Opaque mul : uncps.
+    Hint Rewrite mul_id : uncps.
+
+    Lemma eval_map_multerm s a q (s_nonzero:s<>0): 
+      B.Associational.eval (flat_map (multerm s a) q) = fst a * snd a * B.Associational.eval q.
+    Proof.
+      cbv [multerm multerm_cps Let_In]; induction q;
+      repeat match goal with
+             | _ => progress (autorewrite with uncps push_id cancel_pair push_basesystem_eval in * )
+             | _ => progress simpl flat_map
+             | _ => progress rewrite ?IHq, ?mul_split_mod, ?mul_split_div
+             | _ => rewrite Z.mod_eq by assumption
+             | _ => ring_simplify; omega
+             end.
+    Qed.
+    Hint Rewrite eval_map_multerm using (omega || assumption)
+      : push_basesystem_eval.
+
+    Lemma eval_mul s p q (s_nonzero:s<>0):
+      B.Associational.eval (mul s p q) = B.Associational.eval p * B.Associational.eval q.
+    Proof.
+      cbv [mul mul_cps]; induction p; [reflexivity|].
+      repeat match goal with
+             | _ => progress (autorewrite with uncps push_id push_basesystem_eval in * )
+             | _ => progress simpl flat_map
+             | _ => rewrite IHp
+             | _ => progress change (fun x => multerm_cps s a x id)  with (multerm s a)
+             | _ => ring_simplify; omega
+             end.
+    Qed.
+    Hint Rewrite eval_mul : push_basesystem_eval.
+
+  End Associational.
+End Associational.
+Hint Opaque Associational.mul Associational.multerm : uncps.
+Hint Rewrite @Associational.mul_id @Associational.multerm_id : uncps.
+Hint Rewrite @Associational.eval_mul @Associational.eval_map_multerm : push_basesystem_eval.
+
 Module Columns.
   Section Columns.
     Context (weight : nat->Z)
@@ -316,6 +380,36 @@ Module Columns.
     Proof. apply (proj2 (compact_div_mod inp)). Qed.
     Hint Rewrite @compact_div : push_basesystem_eval.
 
+    (* TODO : move to tuple *)
+    Lemma hd_to_list {A n} a (t : A^(S n)) : List.hd a (to_list (S n) t) = hd t.
+    Proof.
+      rewrite (subst_append t), to_list_append, hd_append. reflexivity.
+    Qed.
+
+    Lemma small_compact {n} x :
+      hd (n:=n) (snd (Columns.compact x)) < weight 1 / weight 0.
+    Proof.
+      match goal with
+        |- ?G => assert (G /\ fst (compact x) = fst (compact x)); [|tauto]
+      end. (* assert a dummy second statement so that fst (compact x) is in context *)
+      cbv [compact compact_cps compact_step compact_step_cps];
+        autorewrite with uncps push_id.
+      change (fun i s a => compact_digit_cps i (s :: a) id)
+      with (fun i s a => compact_digit i (s :: a)).
+      remember (fun i s a => compact_digit i (s :: a)) as f.
+
+      rewrite <-hd_to_list with (a:=0).
+
+      apply @mapi_with'_linvariant with (n:=S n) (start:=0) (f:=f) (inp:=x); intros; try tauto; (split; [|reflexivity]).
+      { let P := fresh "H" in
+        match goal with H : _ /\ _ |- _ => destruct H end.
+        destruct n0; simpl. subst f.
+        { rewrite compact_digit_mod.
+          apply Z.mod_pos_bound, Z.gt_lt, weight_divides. }
+        { rewrite hd_to_list in H1. assumption. } }
+      { simpl. apply Z.gt_lt, weight_divides. }
+    Qed.
+      
     Definition cons_to_nth_cps {n} i (x:Z) (t:(list Z)^n)
                {T} (f:(list Z)^n->T) :=
       @on_tuple_cps _ _ nil (update_nth_cps i (cons x)) n n t _ f.
@@ -424,11 +518,20 @@ Module Columns.
         (fun Q => from_associational_cps weight n (P++Q)
         (fun R => compact_cps (div:=div) (modulo:=modulo) (add_get_carry:=Z.add_get_carry_full) weight R f)))).
 
+    Definition mul_cps {n1 n2 n3 mul_split} s (p : Z^n1) (q : Z^n2)
+               {T} (f : (Z*Z^n3)->T) :=
+      B.Positional.to_associational_cps weight p
+        (fun P => B.Positional.to_associational_cps weight q
+        (fun Q => Associational.mul_cps (mul_split := mul_split) s P Q
+        (fun PQ => from_associational_cps weight n3 PQ
+        (fun R => compact_cps (div:=div) (modulo:=modulo) (add_get_carry:=Z.add_get_carry_full) weight R f)))).
+
     End Wrappers.
 End Columns.
 Hint Unfold
      Columns.add_cps
-     Columns.sub_cps.
+     Columns.sub_cps
+     Columns.mul_cps.
 Hint Rewrite
      @Columns.compact_digit_id
      @Columns.compact_step_id
@@ -586,41 +689,65 @@ Section Freeze.
   Qed.
 End Freeze.
 
-Section API.
-  Context {weight : nat -> Z}
-          {weight_0 : weight 0%nat = 1}
-          {weight_nonzero : forall i, weight i <> 0}
-          {weight_positive : forall i, weight i > 0}
-          {weight_multiples : forall i, weight (S i) mod weight i = 0}
-          {weight_divides : forall i : nat, weight (S i) / weight i > 0}
-  .
+Section UniformWeight.
+  Context (bound : Z) {bound_pos : bound > 0}.
 
+  Definition uweight : nat -> Z := fun i => bound ^ Z.of_nat i.
+  Lemma uweight_0 : uweight 0%nat = 1. Proof. reflexivity. Qed.
+  Lemma uweight_positive i : uweight i > 0.
+  Proof. apply Z.lt_gt, Z.pow_pos_nonneg; omega. Qed.
+  Lemma uweight_nonzero i : uweight i <> 0.
+  Proof. auto using Z.positive_is_nonzero, uweight_positive. Qed.
+  Lemma uweight_multiples i : uweight (S i) mod uweight i = 0.
+  Proof. apply Z.mod_same_pow; rewrite Nat2Z.inj_succ; omega. Qed.
+  Lemma uweight_divides i : uweight (S i) / uweight i > 0.
+  Proof.
+    cbv [uweight]. rewrite <-Z.pow_sub_r by (rewrite ?Nat2Z.inj_succ; omega).
+    apply Z.lt_gt, Z.pow_pos_nonneg; rewrite ?Nat2Z.inj_succ; omega.
+  Qed.
+
+End UniformWeight.
+
+Section API.
+  Context (bound : Z) {bound_pos : bound > 0}.
+  Context {mul_split : Z -> Z -> Z -> Z * Z}
+          {mul_split_mod : forall s x y,
+              fst (mul_split s x y)  = (x * y) mod s}
+          {mul_split_div : forall s x y,
+              snd (mul_split s x y)  = (x * y) / s}.
   Definition T : Type := list Z.
 
-  Definition length : T -> nat := @length Z.
+  Definition numlimbs : T -> nat := @length Z.
 
+  (* lowest limb is less than its bound; this is required for [divmod]
+  to simply separate the lowest limb from the rest and be equivalent
+  to normal div/mod with [bound]. *)
+  Definition small (p : T) : Prop := List.hd 0 p < bound.
+  
   Definition zero (n:nat) : T := to_list _ (B.Positional.zeros n).
   
-  Definition divmod (p : T) : T * Z :=
-    (List.tl p, List.hd 0 p).
+  Definition divmod (p : T) : T * Z := (List.tl p, List.hd 0 p).
 
-  (* TODO : scmul  (Z -> T -> T), using double-output multiply *)
+  Definition drop_high (n : nat) (p : T) : T := firstn n p.
 
-  Definition add (p q : T) : T * Z :=
-    let P := Tuple.from_list (Datatypes.length p) p (eq_refl _) in
-    let Q := Tuple.from_list (Datatypes.length q) q (eq_refl _) in
-    let n := max (Datatypes.length p) (Datatypes.length q) in
-    let carry_result := Columns.add_cps weight P Q id in
-    (to_list n (snd carry_result), fst carry_result).
+  Definition scmul (c : Z) (p : T) : T :=
+    let P := Tuple.from_list (length p) p (eq_refl _) in
+    Columns.mul_cps (mul_split := mul_split) (n1:=1) (n3:=length p) (uweight bound) bound c P
+    (fun carry_result =>
+      to_list _ (left_append (fst carry_result) (snd carry_result))).
 
-  Definition join (to_join : T * Z) : T :=
-    let p := fst to_join in
-    let P := Tuple.from_list (Datatypes.length p) p (eq_refl _) in
-    to_list _ (left_append (snd to_join) P).
-  
+  Definition add (p q : T) : T :=
+    let P := Tuple.from_list (length p) p (eq_refl _) in
+    let Q := Tuple.from_list (length q) q (eq_refl _) in
+    dlet n := max (length p) (length q) in
+    Columns.add_cps (uweight bound) P Q
+      (fun carry_result =>
+        to_list (S n) (left_append (fst carry_result) (snd carry_result))).
+
   Section Proofs.
+    
     Definition eval (p : T) : Z :=
-      B.Positional.eval weight (Tuple.from_list (Datatypes.length p) p (eq_refl _)).
+      B.Positional.eval (uweight bound) (Tuple.from_list (length p) p (eq_refl _)).
 
     Lemma eval_zero n : eval (zero n) = 0.
     Proof.
@@ -631,61 +758,80 @@ Section API.
       Unshelve. distr_length.
     Qed.
 
-    Lemma length_zero n : length (zero n) = n.
+    Lemma numlimbs_zero n : numlimbs (zero n) = n.
     Proof. cbv [eval zero]. apply length_to_list. Qed.
 
+    Local Ltac pose_uweight bound :=
+      match goal with H : bound > 0 |- _ =>
+                      pose proof (uweight_0 bound);
+                      pose proof (@uweight_positive bound H);
+                      pose proof (@uweight_nonzero bound H);
+                      pose proof (@uweight_multiples bound);
+                      pose proof (@uweight_divides bound H)
+      end.
+
     Lemma eval_add_nz p q :
-      max (Datatypes.length p) (Datatypes.length q) <> 0%nat ->
-      eval (fst (add p q)) = eval p + eval q - snd (add p q) * weight (Datatypes.length (fst (add p q))).
+      max (length p) (length q) <> 0%nat ->
+      eval (add p q) = eval p + eval q.
     Proof.
-      intros.
+      intros. pose_uweight bound.
       pose proof Z.add_get_carry_full_div.
       pose proof Z.add_get_carry_full_mod.
       pose proof div_correct. pose proof modulo_correct.
       repeat match goal with
-             | _ => progress (cbv [add eval]; repeat autounfold)
+             | _ => progress (cbv [add eval Let_In]; repeat autounfold)
              | _ => progress autorewrite with uncps push_id cancel_pair push_basesystem_eval
+             | _ => rewrite B.Positional.eval_left_append
+             
              | _ => progress
                       (rewrite <-!from_list_default_eq with (d:=0);
                        erewrite !length_to_list, !from_list_default_eq,
                        from_list_to_list)
-             | _ => rewrite Z.mul_div_eq' by auto using weight_nonzero;
+             | _ => rewrite Z.mul_div_eq by auto;
                       omega
              end.
       Unshelve. distr_length.
     Qed.
 
     Lemma eval_add_z p q :
-      max (Datatypes.length p) (Datatypes.length q) = 0%nat ->
-      eval (fst (add p q)) = eval p + eval q - snd (add p q) * weight (Datatypes.length (fst (add p q))).
+      max (length p) (length q) = 0%nat ->
+      eval (add p q) = eval p + eval q.
     Proof. destruct p, q; distr_length; reflexivity. Qed.
 
-    Lemma eval_add p q : 
-      eval (fst (add p q)) = eval p + eval q - snd (add p q) * weight (Datatypes.length (fst (add p q))).
+    Lemma eval_add p q :  eval (add p q) = eval p + eval q.
     Proof.
-      destruct (Nat.eq_dec (max (Datatypes.length p) (Datatypes.length q)) 0%nat); auto using eval_add_z, eval_add_nz.
+      destruct (Nat.eq_dec (max (length p) (length q)) 0%nat); auto using eval_add_z, eval_add_nz.
     Qed.
     Hint Rewrite eval_add : push_basesystem_eval.
-    
-    Lemma eval_join to_join :
-      eval (join to_join) = eval (fst to_join) + snd to_join * weight (Datatypes.length (fst to_join)).
-    Proof.
-      repeat match goal with
-             | _ => progress (cbv [join eval]; repeat autounfold)
-             | _ => progress autorewrite with uncps push_id cancel_pair push_basesystem_eval
-             | _ => progress
-                      (rewrite <-!from_list_default_eq with (d:=0);
-                       erewrite !length_to_list, !from_list_default_eq,
-                       from_list_to_list)
-             | _ => rewrite B.Positional.eval_left_append; ring_simplify; omega
-             end.
-      Unshelve. distr_length.
-    Qed.
-    Hint Rewrite eval_join : push_basesystem_eval.
 
-    Lemma eval_join_add p q :
-      eval (join (add p q)) = eval p + eval q.
-    Proof. autorewrite with push_basesystem_eval; omega. Qed.
+    Lemma small_add a b : small (add a b).
+    Proof.
+      intros. pose_uweight bound.
+      pose proof Z.add_get_carry_full_div.
+      pose proof Z.add_get_carry_full_mod.
+      pose proof div_correct. pose proof modulo_correct.
+      cbv [small add Let_In]. repeat autounfold.
+      autorewrite with uncps push_id.
+      destruct (max (length a) (length b)); [simpl; omega |].
+      rewrite Columns.hd_to_list, hd_left_append.
+      eapply Z.lt_le_trans.
+      { apply Columns.small_compact; auto. }
+      { cbv [uweight]. simpl Z.of_nat.
+        autorewrite with zsimplify.
+        rewrite Z.pow_1_r. reflexivity. }
+    Qed.
+      
+    Lemma numlimbs_add a b: numlimbs (add a b) = S (max (numlimbs a) (numlimbs b)).
+    Proof.
+    Admitted.
+
+    Lemma eval_scmul a v: eval (scmul a v) = a * eval v.
+    Proof.
+    Admitted.
+      
+    Lemma numlimbs_scmul a v: 0 <= a < bound ->
+                              numlimbs (scmul a v) = S (numlimbs v).
+    Admitted.
 
     (* TODO : move to tuple *)
     Lemma from_list_tl {A n} (ls : list A) H H':
@@ -696,17 +842,31 @@ Section API.
       reflexivity.
     Qed.
     
-    Lemma divmod_div p : eval (fst (divmod p)) = eval p / weight 1.
+    Lemma eval_div p : small p -> eval (fst (divmod p)) = eval p / bound.
     Proof.
       repeat match goal with
-             | _ => progress (cbv [divmod eval]; repeat autounfold)
+             | _ => progress (intros; cbv [divmod eval]; repeat autounfold)
              | _ => progress autorewrite with uncps push_id cancel_pair push_basesystem_eval
              end.
       erewrite from_list_tl.
     Admitted.
     
-    Lemma divmod_mod p : eval (fst (divmod p)) = eval p / weight 1.
+    Lemma eval_mod p : small p -> snd (divmod p) = eval p mod bound.
     Proof.
+    Admitted.
+
+    Lemma small_div v : small v -> small (fst (divmod v)).
+    Admitted.
+
+    Lemma numlimbs_div v : numlimbs (fst (divmod v)) = pred (numlimbs v).
+    Admitted.
+    
+    Lemma eval_drop_high n v :
+      small v -> eval (drop_high n v) = eval v mod (uweight bound n).
+    Admitted.
+    
+    Lemma numlimbs_drop_high n v :
+      numlimbs (drop_high n v) = min (numlimbs v) n.
     Admitted.
       
   End Proofs.
